When flattening cmd.set, don't first create a fresh var to compile the expr into,
and then move value from the fresh var to the target var, but directly compile
the expr into the target var.
Proofs not yet updated at all.
Reduces the number of vars needed for the example to 26

compiler/src/FlattenExpr.v
@@ -69,22 +69,34 @@ Section FlattenExpr1.
   Ltac set_solver :=
     set_solver_generic (@varname p).
 
-  (* returns stmt and var into which result is saved, and new fresh name generator state *)
-  Fixpoint flattenExpr(ngs: NGstate)(e: Syntax.expr):
+  Definition genFresh_if_needed(resVar: option varname)(ngs: NGstate): (varname * NGstate) :=
+    match resVar with
+    | Some r => (r, ngs)
+    | None => genFresh ngs
+    end.
+
+  (* returns stmt and var into which result is saved, and new fresh name generator state.
+     If resVar is not None, the result will be stored there, otherwise a fresh var will
+     be generated for the result if needed (not needed if e already is a var) *)
+  Fixpoint flattenExpr(ngs: NGstate)(resVar: option varname)(e: Syntax.expr):
     (FlatImp.stmt * varname * NGstate) :=
     match e with
     | Syntax.expr.literal n =>
-        let '(x, ngs') := genFresh ngs in
+        let '(x, ngs') := genFresh_if_needed resVar ngs in
         (FlatImp.SLit x n, x, ngs')
-    | Syntax.expr.var x => (FlatImp.SSkip, x, ngs)
+    | Syntax.expr.var x =>
+        match resVar with
+        | Some r => (FlatImp.SSet r x, r, ngs)
+        | None => (FlatImp.SSkip, x, ngs)
+        end
     | Syntax.expr.load sz e =>
-        let '(s1, r1, ngs') := flattenExpr ngs e in
-        let '(x, ngs'') := genFresh ngs' in
+        let '(s1, r1, ngs') := flattenExpr ngs None e in
+        let '(x, ngs'') := genFresh_if_needed resVar ngs' in
         (FlatImp.SSeq s1 (@FlatImp.SLoad (mk_Syntax_params p) sz x r1), x, ngs'')
     | Syntax.expr.op op e1 e2 =>
-        let '(s1, r1, ngs') := flattenExpr ngs e1 in
-        let '(s2, r2, ngs'') := flattenExpr ngs' e2 in
-        let '(x, ngs''') := genFresh ngs'' in
+        let '(s1, r1, ngs') := flattenExpr ngs None e1 in
+        let '(s2, r2, ngs'') := flattenExpr ngs' None e2 in
+        let '(x, ngs''') := genFresh_if_needed resVar ngs'' in
         (FlatImp.SSeq s1
           (FlatImp.SSeq s2
             (@FlatImp.SOp (mk_Syntax_params p) x op r1 r2)), x, ngs''')
@@ -93,11 +105,11 @@ Section FlattenExpr1.
   Definition flattenExprAsBoolExpr(ngs: NGstate)(e: Syntax.expr):
     (FlatImp.stmt * FlatImp.bcond * NGstate) :=
     let default := (* always correct, but in some cases we can do better *)
-        (let '(stmt, x, ngs') := flattenExpr ngs e in (stmt, FlatImp.CondNez x, ngs')) in
+        (let '(stmt, x, ngs') := flattenExpr ngs None e in (stmt, FlatImp.CondNez x, ngs')) in
     match e with
     | Syntax.expr.op op e1 e2 =>
-        let '(s1, r1, ngs') := flattenExpr ngs e1 in
-        let '(s2, r2, ngs'') := flattenExpr ngs' e2 in
+        let '(s1, r1, ngs') := flattenExpr ngs None e1 in
+        let '(s2, r2, ngs'') := flattenExpr ngs' None e2 in
         match op with
         | Syntax.bopname.lts => (FlatImp.SSeq s1 s2, FlatImp.CondBinary FlatImp.BLt  r1 r2, ngs'')
         | Syntax.bopname.ltu => (FlatImp.SSeq s1 s2, FlatImp.CondBinary FlatImp.BLtu r1 r2, ngs'')
@@ -117,7 +129,7 @@ Section FlattenExpr1.
     (FlatImp.stmt * list varname * NGstate) :=
     match es with
     | nil => (FlatImp.SSkip, nil, ngs1)
-    | e :: rest => let '(ci, vi, ngs2) := flattenExpr ngs1 e in
+    | e :: rest => let '(ci, vi, ngs2) := flattenExpr ngs1 None e in
                    let '(cs, vs, ngs3) := flattenExprs ngs2 rest in
                    (FlatImp.SSeq ci cs, vi :: vs, ngs3)
     end.
@@ -139,12 +151,12 @@ Section FlattenExpr1.
   Fixpoint flattenStmt(ngs: NGstate)(s: Syntax.cmd): (FlatImp.stmt * NGstate) :=
     match s with
     | Syntax.cmd.store sz a v =>
-        let '(sa, ra, ngs') := flattenExpr ngs a in
-        let '(sv, rv, ngs'') := flattenExpr ngs' v in
+        let '(sa, ra, ngs') := flattenExpr ngs None a in
+        let '(sv, rv, ngs'') := flattenExpr ngs' None v in
         (FlatImp.SSeq sa (FlatImp.SSeq sv (FlatImp.SStore sz ra rv)), ngs'')
     | Syntax.cmd.set x e =>
-        let '(e', r, ngs') := flattenExpr ngs e in
-        (FlatImp.SSeq e' (FlatImp.SSet x r), ngs')
+        let '(e', x', ngs') := flattenExpr ngs (Some x) e in (* assert(x' = x) *)
+        (e', ngs')
     | Syntax.cmd.cond cond sThen sElse =>
         let '(cond', bcond, ngs') := flattenExprAsBoolExpr ngs cond in
         let '(sThen', ngs'') := flattenStmt ngs' sThen in
@@ -174,10 +186,10 @@ Section FlattenExpr1.
     | _ => idtac
     end.
 
-  Lemma flattenExpr_size: forall e s resVar ngs ngs',
-    flattenExpr ngs e = (s, resVar, ngs') ->
+  Lemma flattenExpr_size: forall e s oResVar resVar ngs ngs',
+    flattenExpr ngs oResVar e = (s, resVar, ngs') ->
     0 <= FlatImp.stmt_size s <= 2 * ExprImp.expr_size e.
-  Proof.
+  Proof. Admitted. (*
     induction e; intros; simpl in *; simp; simpl; try omega.
     - specializes IHe; [eassumption|]. omega.
     - specializes IHe1; [eassumption|].
@@ -954,6 +966,7 @@ map_solver locals_ok.
   Qed.
 *)
   Admitted.
+  *)
 
   Definition ExprImp2FlatImp(s: Syntax.cmd): FlatImp.stmt :=
     fst (flattenStmt (freshNameGenState (ExprImp.allVars_cmd s)) s).
@@ -965,6 +978,7 @@ map_solver locals_ok.
         post t' m' lH' /\
         map.extends lL' lH').
   Proof.
+  Admitted. (*
     intros.
     unfold ExprImp2FlatImp in *.
     match goal with
@@ -986,5 +1000,6 @@ map_solver locals_ok.
         specialize Q with (1 := H). exact Q.
     - simpl. intros. simp. eauto.
   Qed.
+  *)
 
 End FlattenExpr1.
